model

src/Distributions/Geometric/Model.dfy
@@ -5,30 +5,54 @@
 
 include "../../ProbabilisticProgramming/Monad.dfy"
 include "../../ProbabilisticProgramming/WhileAndUntil.dfy"
+include "../../ProbabilisticProgramming/Independence.dfy"
+include "../../ProbabilisticProgramming/Quantifier.dfy"
 
 module GeometricModel {
   import Monad
   import WhileAndUntil
+  import Independence
+  import Quantifier
 
   // Equation (4.18)
   function Sample(): Monad.Hurd<int> {
     var fst := (t: (bool, int)) => t.0;
     var f := (t: (bool, int)) => Monad.Return(t.1 - 1);
     ProbWhileGeometricTerminates();
-    var g := WhileAndUntil.ProbWhile(fst, GeometricIter, (true, 0));
+    var g := WhileAndUntil.ProbWhile(fst, SampleIter, (true, 0));
     Monad.Bind(g, f)
   }
 
   // Equation (4.17)
-  function GeometricIter(t: (bool, int)): (f: Monad.Hurd<(bool, int)>)
+  function SampleIter(t: (bool, int)): (f: Monad.Hurd<(bool, int)>)
     ensures forall s :: f(s) == ((Monad.Head(s), t.1 + 1), Monad.Tail(s))
+    ensures Independence.IsIndepFn(f)
   {
-    Monad.Bind(Monad.Deconstruct, (b': bool) => Monad.Return((b', t.1 + 1)))
+    var g := (b': bool) => Monad.Return((b', t.1 + 1));
+    assert forall b' :: Independence.IsIndepFn(g(b')) by {
+      forall b' ensures Independence.IsIndepFn(g(b')) {
+        Independence.ReturnIsIndepFn((b', t.1 + 1));
+      }
+    }
+    var f := Monad.Bind(Monad.Deconstruct, g);
+    assert Independence.IsIndepFn(f) by {
+      Independence.DeconstructIsIndepFn();
+      Independence.IndepFnIsCompositional(Monad.Deconstruct, g);
+    }
+    f
   }
 
-  lemma {:axiom} ProbWhileGeometricTerminates()
+  lemma ProbWhileGeometricTerminates()
     ensures
       var fst := (t: (bool, int)) => t.0;
-      WhileAndUntil.ProbWhileTerminates(GeometricIter, fst)
+      WhileAndUntil.ProbWhileTerminates(SampleIter, fst)
+  {
+    var fst := (t: (bool, int)) => t.0;
+    assert forall t :: Independence.IsIndepFn(SampleIter(t));
+    assert forall t :: Quantifier.ExistsStar(WhileAndUntil.Helper(SampleIter, fst, t)) by {
+      assume {:axiom} false;
+    }
+    WhileAndUntil.EnsureProbWhileTerminates(SampleIter, fst);
+  }
 
 }
